Safety.v
@@ -40,11 +40,61 @@ Definition is_instr_class_safe (s : state) (i : instr_class) : bool :=
 | _ => true
 end.
 
+Inductive safe_instr_class : instr_class -> state -> Prop :=
+| I_Heap_Read_Safe: forall r_dst r_src r_base st,
+  Word.eq (get_register st r_base) (st.(heap_base)) = true ->
+  Word.lt (get_register st r_src) fourGB =  true ->
+  safe_instr_class (Heap_Read r_dst r_src r_base) st
+| I_Heap_Write_Safe: forall r_dst r_val r_base st,
+  Word.eq (get_register st r_base) (st.(heap_base)) = true ->
+  Word.lt (get_register st r_dst) fourGB =  true ->
+  safe_instr_class (Heap_Write r_dst r_val r_base) st
+| I_Heap_Check_Safe: forall reg st,
+  safe_instr_class (Heap_Check reg) st
+| I_CF_Check_Safe: forall reg st,
+  safe_instr_class (CF_Check reg) st
+| I_Reg_Move_Safe: forall r_dst r_src st,
+  safe_instr_class (Reg_Move r_dst r_src) st
+| I_Reg_Write_Safe: forall r_dst val st,
+  safe_instr_class (Reg_Write r_dst val) st
+| I_Stack_Expand_Safe: forall st i,
+  safe_instr_class (Stack_Expand i) st
+| I_Stack_Contract_Safe: forall st i,
+  i <= length st.(stack) ->
+  safe_instr_class (Stack_Contract i) st
+| I_Stack_Read_Safe: forall st i r_dst,
+  i < length st.(stack) ->
+  safe_instr_class (Stack_Read r_dst i) st
+| I_Stack_Write_Safe: forall st i r_src,
+  i < length st.(stack) ->
+  safe_instr_class (Stack_Write i r_src) st
+| I_Indirect_Call_Safe: forall st reg,
+  Word.eq (get_register st rdi) st.(heap_base) = true ->
+  member st.(function_table) (get_register st reg) = true ->
+  safe_instr_class (Indirect_Call reg) st
+| I_Direct_Call_Safe: forall st,
+  Word.eq (get_register st rdi) st.(heap_base) = true ->
+  safe_instr_class (Direct_Call) st
+| I_Ret_Safe: forall st,
+  length st.(stack) = 0 ->
+  safe_instr_class (Ret) st.
+
+(*
 Fixpoint is_basic_block_safe (s : state) (bb : basic_block) : bool :=
 match bb with
 | nil => true
 | i :: bb' => andb (is_instr_class_safe s i) (is_basic_block_safe (run_instr i s) bb') 
 end.
+*)
+
+Inductive safe_basic_block : basic_block -> state -> Prop :=
+| I_Basic_Block_Empty_Safe : forall st,
+  safe_basic_block nil st
+| I_Basic_Block_Cons_Safe : forall i bb st st',
+  safe_instr_class i st ->
+  instr_class_istep i st st' ->
+  safe_basic_block bb st' ->
+  safe_basic_block (i :: bb) st.
 
 Definition abstractify_int64 (s : state) (i : int64) : info :=
 if (Word.eq i s.(heap_base)) then mem_base else
@@ -105,10 +155,43 @@ Proof.
     * remember (Word.lt i fourGB) as not_goal. destruct not_goal; inversion H.
 Qed.
 
+Theorem instr_class_vstep_safe : forall i abs_st abs_st' st,
+  abs_st = abstractify st ->
+  i / abs_st v--> abs_st' -> 
+  safe_instr_class i st.
+Proof.
+  intros i abs_st abs_st' st Hst Hstep. induction Hstep; subst.
+- apply I_Heap_Read_Safe. 
+  + inversion H0. unfold abstractify_registers, abstractify_int64 in H2. apply safe_mem_base; auto.
+  + inversion H0. unfold abstractify_registers, abstractify_int64 in H2. apply safe_mem_bound in H2; auto.
+- apply I_Heap_Write_Safe.
+  + inversion H0. unfold abstractify_registers, abstractify_int64 in H2. apply safe_mem_base; auto.
+  + inversion H0. unfold abstractify_registers, abstractify_int64 in H2. apply safe_mem_bound in H2; auto.
+- apply I_Heap_Check_Safe.
+- apply I_CF_Check_Safe.
+- apply I_Reg_Move_Safe.
+- apply I_Reg_Write_Safe.
+- apply I_Stack_Expand_Safe.
+- apply I_Stack_Contract_Safe.
+  unfold abstractify, abstractify_list in H. simpl in H.
+  rewrite <- map_length with (f := abstractify_int64 st). auto.
+- apply I_Stack_Read_Safe. unfold abstractify, abstractify_list in H. simpl in H.
+  rewrite <- map_length with (f := abstractify_int64 st). auto.
+- apply I_Stack_Write_Safe. unfold abstractify, abstractify_list in H. simpl in H.
+  rewrite <- map_length with (f := abstractify_int64 st). auto.
+- apply I_Indirect_Call_Safe.
+  + inversion H0. unfold abstractify_registers, abstractify_int64 in H2. apply safe_mem_base; auto.
+  + inversion H. unfold abstractify_registers, abstractify_int64 in H2. apply safe_function_index; auto.
+- apply I_Direct_Call_Safe.
+  inversion H. unfold abstractify_registers, abstractify_int64 in H1. apply safe_mem_base; auto.
+- apply I_Ret_Safe.
+  inversion H. unfold abstractify_list in H1. apply map_eq_nil in H1. rewrite H1. auto.
+Qed.
+
 Theorem safe_instr : 
   forall i abs_st abs_st' st,
     abs_st = abstractify st ->
-    instr_class_flow_function i abs_st abs_st' ->
+    instr_class_vstep i abs_st abs_st' ->
     is_instr_class_safe st i = true.
 Proof.
   intros i abs_st abst_st' st Hst Hstep. unfold is_instr_class_safe, is_mem_bounded. induction Hstep; subst; auto.
@@ -139,19 +222,52 @@ Proof.
   apply map_eq_nil in H. apply PeanoNat.Nat.eqb_eq. rewrite H. auto.
 Qed.
 
-Theorem safe_basic_block : 
+(*
+Lemma basic_helper : forall a bb abs_st abs_st' abs_st'', 
+multi basic_block_flow_function (a :: bb, abs_st) (nil, abs_st'') ->
+   basic_block_flow_function (a :: bb, abs_st) (bb, abs_st') 
+/\ multi basic_block_flow_function (bb, abs_st') (nil, abs_st'').
+Proof.
+  
+  intros. eapply multi_step in H. induction a.
+- inversion H. inversion H0. inversion H1. subst. split.
+
+ inversion H. inversion H0. inversion H1. subst. induction a; inversion H; subst.
+- inversion H0. inversion H1. subst. split. apply I_Basic_Block. inversion H8. subst. auto.
+  +
+*)
+
+Theorem instr_class_istep_abstractify_vstep: forall i st st' abs_st',
+  i / abstractify st v--> abs_st' ->
+  i / st i--> st' ->
+  abs_st' = abstractify st'.
+Proof.
+  intros i st st' abs_st' Hv Hi. induction i; inversion Hv; inversion Hi; subst.
+- unfold get_register_info, set_register_info in *. unfold map_get, map_set in *.
+  unfold set_register, abstractify, abstractify_registers. simpl. unfold map_set. simpl. unfold abstractify_list.
+  simpl. unfold abstractify_int64. simpl. admit.
+- admit.
+- unfold abstractify. simpl. unfold set_register_info. simpl.
+unfold set_register, set_register_info, abstractify. simpl. unfold abstractify_registers. unfold map_set. simpl.
+  unfold abstractify_int64. simpl.
+Admitted.
+  
+Theorem basic_block_vstep_safe : 
   forall bb abs_st abs_st' st,
   abs_st = abstractify st ->
-  multi_basic_block_flow_function (bb, abs_st) (nil, abs_st') ->
-  is_basic_block_safe st bb = true.
+  multi_basic_block_vstep (bb, abs_st) (nil, abs_st') ->
+  safe_basic_block bb st.
 Proof.
   intros bb abs_st abs_st' st Hst Hstep. generalize dependent abs_st. generalize dependent st. induction bb.
-  - auto.
-  - simpl. intros st abs_st Hst Hstep. apply andb_true_intro. split.
-    + inversion Hstep. inversion H. eapply safe_instr. apply Hst. apply H7.
-    + inversion Hstep. apply IHbb with (st := (run_instr a st)) (abs_st := abstractify (run_instr a st)). auto.
-      auto.
-      * unfold abstractify. unfold abstractify_registers, abstractify_list. simpl. 
-
- apply Hst. apply IHbb'. inversion Hstep. apply IHbb. 
-
+- intros st abs_st Hst Hstep. apply I_Basic_Block_Empty_Safe.
+- intros st abs_st Hst Hstep. inversion Hstep; subst.  inversion H; subst.
+  assert (exists st'', a / st i--> st'').
+{ apply instr_class_always_isteps. }
+  inversion H1. 
+  apply I_Basic_Block_Cons_Safe with (st' := x).
+  + apply instr_class_vstep_safe with (abs_st := abstractify st) (abs_st' := st'); auto.
+  + auto.
+  + apply IHbb with (abs_st := st').
+    * eapply instr_class_istep_abstractify_vstep. apply H5. apply H2.
+    * auto.
+Qed.
